compiler/backend/data_to_wordScript.sml
@@ -1618,10 +1618,17 @@ val def = assign_Define `
 
 val def = assign_Define `
   assign_WordTest (l:num) (dest:num) (test: ast$test) v1 v2 =
-                 (If (dtcase test of Equal => Equal | _ => Lower)
-                   (adjust_var v1) (Reg (adjust_var v2))
-                   (Assign (adjust_var dest) TRUE_CONST)
-                   (Assign (adjust_var dest) FALSE_CONST),l)
+       ((dtcase test of
+         | Equal  => If Equal (adjust_var v1) (Reg (adjust_var v2))
+                        (Assign (adjust_var dest) TRUE_CONST)
+                        (Assign (adjust_var dest) FALSE_CONST)
+         | Less   => If Lower (adjust_var v1) (Reg (adjust_var v2))
+                       (Assign (adjust_var dest) TRUE_CONST)
+                       (Assign (adjust_var dest) FALSE_CONST)
+         | LessEq => If NotLower (adjust_var v2) (Reg (adjust_var v1))
+                       (Assign (adjust_var dest) TRUE_CONST)
+                       (Assign (adjust_var dest) FALSE_CONST)
+         | _      => Skip),l)
       : 'a wordLang$prog # num`;
 
 val def = assign_Define `
