compiler/backend/proofs/data_to_word_assignProofScript.sml
@@ -9150,7 +9150,9 @@ Proof
     gvs [Smallnum_def,INT_EQ_NUM_LEMMA,dimword_def,good_dimindex_def]
   \\ ‘(Smallnum n1' <+ Smallnum n2' :α word) ⇔  (n1' < n2')’ by
     gvs [Smallnum_def,INT_EQ_NUM_LEMMA,dimword_def,good_dimindex_def,WORD_LO]
-  \\ simp []
+  \\ ‘(Smallnum n1' <=+ Smallnum n2' :α word) ⇔  (n1' <= n2')’ by
+    gvs [Smallnum_def,INT_EQ_NUM_LEMMA,dimword_def,good_dimindex_def,WORD_LS]
+  \\ simp [] \\ fs [GSYM WORD_NOT_LOWER]
   \\ IF_CASES_TAC \\ gvs [wordSemTheory.word_exp_def,wordSemTheory.set_var_def]
   \\ fs [] \\ fs [lookup_insert,adjust_var_11] \\ rw [] \\ fs []
   \\ simp[inter_insert_ODD_adjust_set,GSYM Boolv_def,option_le_max_right]
